some prog fixes, derived lock specs from atomic locks

progs/incr.c
@@ -1,39 +1,38 @@
 #include "../concurrency/threads.h"
 //#include <stdio.h>
 
-lock_t *ctr_lock;
-lock_t *thread_lock;
-unsigned ctr;
+typedef struct counter { unsigned ctr; lock_t *lock; } counter;
+counter c;
 
 void incr() {
-  acquire(ctr_lock);
-  ctr = ctr + 1;
-  release(ctr_lock);
+  acquire(c.lock);
+  c.ctr = c.ctr + 1;
+  release(c.lock);
 }
 
 unsigned read() {
-  acquire(ctr_lock);
-  unsigned t = ctr;
-  release (ctr_lock);
+  acquire(c.lock);
+  unsigned t = c.ctr;
+  release (c.lock);
   return t;
 }
 
-int thread_func(void *args) {
+int thread_func(void *thread_lock) {
   //Increment the counter
   incr();
   //Yield: 'ready to join'.
-  release2(thread_lock);
+  release((lock_t *)thread_lock);
   return 0;
 }
 
 int main(void)
 {
-  ctr = 0;
-  ctr_lock = makelock();
-  release(ctr_lock);
-  thread_lock = makelock();
+  c.ctr = 0;
+  c.lock = makelock();
+  release(c.lock);
+  lock_t *thread_lock = makelock();
   /* Spawn */
-  spawn((void *)&thread_func, (void *)NULL);
+  spawn((void *)&thread_func, (void *)thread_lock);
 
   //Increment the counter
   incr();
@@ -41,10 +40,10 @@ int main(void)
   /*JOIN */
   acquire(thread_lock);
   unsigned t = read();
-  acquire(ctr_lock);
+  acquire(c.lock);
   /* free the locks */
-  freelock2(thread_lock);
-  freelock(ctr_lock);
+  freelock(thread_lock);
+  freelock(c.lock);
 
   /*printf("I'm done with a final counter of: %d\n", t);*/
 
