atomics/general_atomics.v
@@ -25,7 +25,7 @@ Lemma atomic_commit_fupd : forall {A B} (a : A -> mpred) Eo Ei (b : A -> B -> mp
 Proof.
   intros.
   iIntros "[AS R]".
-  unfold atomic_shift.
+  unfold atomic_shift. 
   iMod "AS" as (x) "[a [_ commit]]"; simpl.
   iMod (H with "[$R $a]") as (y) "[b Q]".
   iExists y; iMod ("commit" with "b") as "$"; auto.
@@ -628,7 +628,7 @@ Notation "'ATOMIC' 'TYPE' W 'OBJ' x 'INVS' E 'WITH' x1 , .. , xn 'PRE'  [ u , ..
      (PARAMSx (cons Lx%type .. (cons Ly%type nil) ..) (GLOBALSx (cons Gx .. (cons Gy nil) ..)
      (SEPx (cons (atomic_shift(B := unit) (fun x => S2) (⊤ ∖ E) ∅ (fun x _ => fold_right_sepcon (cons SQx%logic .. (cons SQy%logic nil) ..)) (fun _ => Q)) (cons S1x%logic .. (cons S1y%logic nil) ..)))))))) ..)))
    (fun (ts: list Type) => rev_curry (tcurry (fun x1 => .. (tcurry (fun xn => tcurry (fun (Q : mpred) (_ : tuple_type tnil) =>
-     PROP () LOCAL () (SEPx (Q :: cons SPx .. (cons SPy nil) ..))))) ..)))
+     PROP () (LOCALx (cons LQx .. (cons LQy nil) ..) (SEPx (Q :: cons SPx .. (cons SPy nil) ..)))))) ..)))
    (@atomic_spec_nonexpansive_pre0 _ W
       (fun (ts: list Type) => rev_curry (tcurry (fun x1 => .. (tcurry (fun xn (_ : tuple_type tnil) => (cons Px%type .. (cons Py%type nil) ..))) ..)))
       (fun (ts: list Type) => rev_curry (tcurry (fun x1 => .. (tcurry (fun xn (_ : tuple_type tnil) => (cons Lx%type .. (cons Ly%type nil) ..))) ..)))
@@ -638,8 +638,8 @@ Notation "'ATOMIC' 'TYPE' W 'OBJ' x 'INVS' E 'WITH' x1 , .. , xn 'PRE'  [ u , ..
       (fun (ts: list Type) => rev_curry (tcurry (fun x1 => .. (tcurry (fun xn (_ : tuple_type tnil) x _ => fold_right_sepcon (cons SQx%logic .. (cons SQy%logic nil) ..))) ..)))
      _ _ _ _ _ _)
   (atomic_spec_nonexpansive_post0 W
-      (fun (ts: list Type) => rev_curry (tcurry (fun x1 => .. (tcurry (fun xn (_ : tuple_type tnil) => (cons LQx%logic .. (cons LQy%logic nil) ..))) ..)))
-      (fun (ts: list Type) => rev_curry (tcurry (fun x1 => .. (tcurry (fun xn (_ : tuple_type tnil) => (cons SPx%assert5%assert3 .. (cons SPy%assert5%assert3 nil) ..))) ..))) _ _))
+      (fun (ts: list Type) => rev_curry (tcurry (fun x1 => .. (tcurry (fun xn (_ : tuple_type tnil) => (cons LQx%assert3 .. (cons LQy%assert3 nil) ..))) ..)))
+      (fun (ts: list Type) => rev_curry (tcurry (fun x1 => .. (tcurry (fun xn (_ : tuple_type tnil) => (cons SPx%assert3 .. (cons SPy%assert3 nil) ..))) ..))) _ _))
   (at level 200, x1 closed binder, xn closed binder, x at level 0, E at level 0, S2 at level 0).
 
 Notation "'ATOMIC' 'TYPE' W 'OBJ' x 'INVS' E 'WITH' x1 , .. , xn 'PRE'  [ u , .. , v ] 'PROP' ( Px ; .. ; Py ) 'PARAMS' ( Lx ; .. ; Ly ) 'GLOBALS' ( Gx ; .. ; Gy ) 'SEP' ( S1x ; .. ; S1y ) '|' S2 'POST' [ tz ] 'PROP' () 'LOCAL' () 'SEP' ( SPx ; .. ; SPy ) '|' ( SQx ; .. ; SQy )" :=
@@ -714,7 +714,7 @@ Notation "'ATOMIC' 'TYPE' W 'OBJ' x 'INVS' E 'WITH' x1 , .. , xn 'PRE'  [ ] 'PRO
      (PARAMSx (cons Lx%type .. (cons Ly%type nil) ..) (GLOBALSx (cons Gx .. (cons Gy nil) ..)
      (SEPx (cons (atomic_shift(B := unit) (fun x => S2) (⊤ ∖ E) ∅ (fun x _ => fold_right_sepcon (cons SQx%logic .. (cons SQy%logic nil) ..)) (fun _ => Q)) (cons S1x%logic .. (cons S1y%logic nil) ..)))))))) ..)))
    (fun (ts: list Type) => rev_curry (tcurry (fun x1 => .. (tcurry (fun xn => tcurry (fun (Q : mpred) (_ : tuple_type tnil) =>
-     PROP () LOCAL () (SEPx (Q :: cons SPx .. (cons SPy nil) ..))))) ..)))
+     PROP () (LOCALx (cons LQx .. (cons LQy nil) ..) (SEPx (Q :: cons SPx .. (cons SPy nil) ..)))))) ..)))
    (@atomic_spec_nonexpansive_pre0 _ W
       (fun (ts: list Type) => rev_curry (tcurry (fun x1 => .. (tcurry (fun xn (_ : tuple_type tnil) => (cons Px%type .. (cons Py%type nil) ..))) ..)))
       (fun (ts: list Type) => rev_curry (tcurry (fun x1 => .. (tcurry (fun xn (_ : tuple_type tnil) => (cons Lx%type .. (cons Ly%type nil) ..))) ..)))
@@ -724,8 +724,8 @@ Notation "'ATOMIC' 'TYPE' W 'OBJ' x 'INVS' E 'WITH' x1 , .. , xn 'PRE'  [ ] 'PRO
       (fun (ts: list Type) => rev_curry (tcurry (fun x1 => .. (tcurry (fun xn (_ : tuple_type tnil) x _ => fold_right_sepcon (cons SQx%logic .. (cons SQy%logic nil) ..))) ..)))
      _ _ _ _ _ _)
   (atomic_spec_nonexpansive_post0 W
-      (fun (ts: list Type) => rev_curry (tcurry (fun x1 => .. (tcurry (fun xn (_ : tuple_type tnil) => (cons LQx%logic .. (cons LQy%logic nil) ..))) ..)))
-      (fun (ts: list Type) => rev_curry (tcurry (fun x1 => .. (tcurry (fun xn (_ : tuple_type tnil) => (cons SPx%assert5%assert3 .. (cons SPy%assert5%assert3 nil) ..))) ..))) _ _))
+      (fun (ts: list Type) => rev_curry (tcurry (fun x1 => .. (tcurry (fun xn (_ : tuple_type tnil) => (cons LQx%assert3 .. (cons LQy%assert3 nil) ..))) ..)))
+      (fun (ts: list Type) => rev_curry (tcurry (fun x1 => .. (tcurry (fun xn (_ : tuple_type tnil) => (cons SPx%assert3 .. (cons SPy%assert3 nil) ..))) ..))) _ _))
   (at level 200, x1 closed binder, xn closed binder, x at level 0, E at level 0, S2 at level 0).
 
 Notation "'ATOMIC' 'TYPE' W 'OBJ' x 'INVS' E 'WITH' x1 , .. , xn 'PRE'  [ ] 'PROP' ( Px ; .. ; Py ) 'PARAMS' ( Lx ; .. ; Ly ) 'GLOBALS' ( Gx ; .. ; Gy ) 'SEP' ( S1x ; .. ; S1y ) '|' S2 'POST' [ tz ] 'PROP' () 'LOCAL' () 'SEP' ( SPx ; .. ; SPy ) '|' ( SQx ; .. ; SQy )" :=
@@ -800,7 +800,7 @@ Notation "'ATOMIC' 'TYPE' W 'OBJ' x 'INVS' E 'WITH' x1 , .. , xn 'PRE'  [ u , ..
      (PARAMSx nil (GLOBALSx (cons Gx .. (cons Gy nil) ..)
      (SEPx (cons (atomic_shift(B := unit) (fun x => S2) (⊤ ∖ E) ∅ (fun x _ => fold_right_sepcon (cons SQx%logic .. (cons SQy%logic nil) ..)) (fun _ => Q)) (cons S1x%logic .. (cons S1y%logic nil) ..)))))))) ..)))
    (fun (ts: list Type) => rev_curry (tcurry (fun x1 => .. (tcurry (fun xn => tcurry (fun (Q : mpred) (_ : tuple_type tnil) =>
-     PROP () LOCAL () (SEPx (Q :: cons SPx .. (cons SPy nil) ..))))) ..)))
+     PROP () (LOCALx (cons LQx .. (cons LQy nil) ..) (SEPx (Q :: cons SPx .. (cons SPy nil) ..)))))) ..)))
    (@atomic_spec_nonexpansive_pre0 _ W
       (fun (ts: list Type) => rev_curry (tcurry (fun x1 => .. (tcurry (fun xn (_ : tuple_type tnil) => (cons Px%type .. (cons Py%type nil) ..))) ..)))
       (fun (ts: list Type) => rev_curry (tcurry (fun x1 => .. (tcurry (fun xn (_ : tuple_type tnil) => nil)) ..)))
@@ -810,8 +810,8 @@ Notation "'ATOMIC' 'TYPE' W 'OBJ' x 'INVS' E 'WITH' x1 , .. , xn 'PRE'  [ u , ..
       (fun (ts: list Type) => rev_curry (tcurry (fun x1 => .. (tcurry (fun xn (_ : tuple_type tnil) x _ => fold_right_sepcon (cons SQx%logic .. (cons SQy%logic nil) ..))) ..)))
      _ _ _ _ _ _)
   (atomic_spec_nonexpansive_post0 W
-      (fun (ts: list Type) => rev_curry (tcurry (fun x1 => .. (tcurry (fun xn (_ : tuple_type tnil) => (cons LQx%logic .. (cons LQy%logic nil) ..))) ..)))
-      (fun (ts: list Type) => rev_curry (tcurry (fun x1 => .. (tcurry (fun xn (_ : tuple_type tnil) => (cons SPx%assert5%assert3 .. (cons SPy%assert5%assert3 nil) ..))) ..))) _ _))
+      (fun (ts: list Type) => rev_curry (tcurry (fun x1 => .. (tcurry (fun xn (_ : tuple_type tnil) => (cons LQx%assert3 .. (cons LQy%assert3 nil) ..))) ..)))
+      (fun (ts: list Type) => rev_curry (tcurry (fun x1 => .. (tcurry (fun xn (_ : tuple_type tnil) => (cons SPx%assert3 .. (cons SPy%assert3 nil) ..))) ..))) _ _))
   (at level 200, x1 closed binder, xn closed binder, x at level 0, E at level 0, S2 at level 0).
 
 Notation "'ATOMIC' 'TYPE' W 'OBJ' x 'INVS' E 'WITH' x1 , .. , xn 'PRE'  [ u , .. , v ] 'PROP' ( Px ; .. ; Py ) 'PARAMS' () 'GLOBALS' ( Gx ; .. ; Gy ) 'SEP' ( S1x ; .. ; S1y ) '|' S2 'POST' [ tz ] 'PROP' () 'LOCAL' () 'SEP' ( SPx ; .. ; SPy ) '|' ( SQx ; .. ; SQy )" :=
@@ -879,14 +879,14 @@ Notation "'ATOMIC' 'TYPE' W 'OBJ' x 'INVS' E 'WITH' x1 , .. , xn 'PRE'  [ ] 'PRO
       (fun (ts: list Type) => rev_curry (tcurry (fun x1 => .. (tcurry (fun xn (_ : tuple_type tnil) r => (cons SPx%assert5%assert3 .. (cons SPy%assert5%assert3 nil) ..))) ..))) _ _))
   (at level 200, x1 closed binder, xn closed binder, x at level 0, E at level 0, S2 at level 0, r at level 0, T at level 0).
 
-Notation "'ATOMIC' 'TYPE' W 'OBJ' x 'INVS' E 'WITH' x1 , .. , xn 'PRE'  [ ] 'PROP' ( Px ; .. ; Py ) 'PARAMS () 'GLOBALS' ( Gx ; .. ; Gy ) 'SEP' ( S1x ; .. ; S1y ) '|' S2 'POST' [ tz ] 'PROP' () 'LOCAL' ( LQx ; .. ; LQy ) 'SEP' ( SPx ; .. ; SPy ) '|' ( SQx ; .. ; SQy )" :=
+Notation "'ATOMIC' 'TYPE' W 'OBJ' x 'INVS' E 'WITH' x1 , .. , xn 'PRE'  [ ] 'PROP' ( Px ; .. ; Py ) 'PARAMS' () 'GLOBALS' ( Gx ; .. ; Gy ) 'SEP' ( S1x ; .. ; S1y ) '|' S2 'POST' [ tz ] 'PROP' () 'LOCAL' ( LQx ; .. ; LQy ) 'SEP' ( SPx ; .. ; SPy ) '|' ( SQx ; .. ; SQy )" :=
   (mk_funspec (pair nil tz) cc_default (atomic_spec_type0 W)
    (fun (ts: list Type) => rev_curry (tcurry (fun x1 => .. (tcurry (fun xn => tcurry (fun (Q : mpred) (_ : tuple_type tnil) =>
      PROPx (cons Px%type .. (cons Py%type nil) ..)
      (PARAMSx nil (GLOBALSx (cons Gx .. (cons Gy nil) ..)
      (SEPx (cons (atomic_shift(B := unit) (fun x => S2) (⊤ ∖ E) ∅ (fun x _ => fold_right_sepcon (cons SQx%logic .. (cons SQy%logic nil) ..)) (fun _ => Q)) (cons S1x%logic .. (cons S1y%logic nil) ..)))))))) ..)))
    (fun (ts: list Type) => rev_curry (tcurry (fun x1 => .. (tcurry (fun xn => tcurry (fun (Q : mpred) (_ : tuple_type tnil) =>
-     PROP () LOCAL () (SEPx (Q :: cons SPx .. (cons SPy nil) ..))))) ..)))
+     PROP () (LOCALx (cons LQx .. (cons LQy nil) ..) (SEPx (Q :: cons SPx .. (cons SPy nil) ..)))))) ..)))
    (@atomic_spec_nonexpansive_pre0 _ W
       (fun (ts: list Type) => rev_curry (tcurry (fun x1 => .. (tcurry (fun xn (_ : tuple_type tnil) => (cons Px%type .. (cons Py%type nil) ..))) ..)))
       (fun (ts: list Type) => rev_curry (tcurry (fun x1 => .. (tcurry (fun xn (_ : tuple_type tnil) => nil)) ..)))
@@ -896,8 +896,8 @@ Notation "'ATOMIC' 'TYPE' W 'OBJ' x 'INVS' E 'WITH' x1 , .. , xn 'PRE'  [ ] 'PRO
       (fun (ts: list Type) => rev_curry (tcurry (fun x1 => .. (tcurry (fun xn (_ : tuple_type tnil) x _ => fold_right_sepcon (cons SQx%logic .. (cons SQy%logic nil) ..))) ..)))
      _ _ _ _ _ _)
   (atomic_spec_nonexpansive_post0 W
-      (fun (ts: list Type) => rev_curry (tcurry (fun x1 => .. (tcurry (fun xn (_ : tuple_type tnil) => (cons LQx%logic .. (cons LQy%logic nil) ..))) ..)))
-      (fun (ts: list Type) => rev_curry (tcurry (fun x1 => .. (tcurry (fun xn (_ : tuple_type tnil) => (cons SPx%assert5%assert3 .. (cons SPy%assert5%assert3 nil) ..))) ..))) _ _))
+      (fun (ts: list Type) => rev_curry (tcurry (fun x1 => .. (tcurry (fun xn (_ : tuple_type tnil) => (cons LQx%assert3 .. (cons LQy%assert3 nil) ..))) ..)))
+      (fun (ts: list Type) => rev_curry (tcurry (fun x1 => .. (tcurry (fun xn (_ : tuple_type tnil) => (cons SPx%assert3 .. (cons SPy%assert3 nil) ..))) ..))) _ _))
   (at level 200, x1 closed binder, xn closed binder, x at level 0, E at level 0, S2 at level 0).
 
 Notation "'ATOMIC' 'TYPE' W 'OBJ' x 'INVS' E 'WITH' x1 , .. , xn 'PRE'  [ ] 'PROP' ( Px ; .. ; Py ) 'PARAMS' () 'GLOBALS' ( Gx ; .. ; Gy ) 'SEP' ( S1x ; .. ; S1y ) '|' S2 'POST' [ tz ] 'PROP' () 'LOCAL' () 'SEP' ( SPx ; .. ; SPy ) '|' ( SQx ; .. ; SQy )" :=
@@ -919,6 +919,48 @@ Notation "'ATOMIC' 'TYPE' W 'OBJ' x 'INVS' E 'WITH' x1 , .. , xn 'PRE'  [ ] 'PRO
   (atomic_spec_nonexpansive_post0 W
       (fun (ts: list Type) => rev_curry (tcurry (fun x1 => .. (tcurry (fun xn (_ : tuple_type tnil) => nil)) ..)))
       (fun (ts: list Type) => rev_curry (tcurry (fun x1 => .. (tcurry (fun xn (_ : tuple_type tnil) => (cons SPx%assert5%assert3 .. (cons SPy%assert5%assert3 nil) ..))) ..))) _ _))
+  (at level 200, x1 closed binder, xn closed binder, x at level 0, E at level 0, S2 at level 0).
+
+Notation "'ATOMIC' 'TYPE' W 'OBJ' x 'INVS' E 'WITH' x1 , .. , xn 'PRE'  [ ] 'PROP' () 'PARAMS' () 'GLOBALS' ( Gx ; .. ; Gy ) 'SEP' () '|' S2 'POST' [ tz ] 'PROP' () 'LOCAL' ( LQx ; .. ; LQy ) 'SEP' () '|' ( SQx ; .. ; SQy )" :=
+  (mk_funspec (pair nil tz) cc_default (atomic_spec_type0 W)
+   (fun (ts: list Type) => rev_curry (tcurry (fun x1 => .. (tcurry (fun xn => tcurry (fun (Q : mpred) (_ : tuple_type tnil) =>
+     PROPx nil
+     (PARAMSx nil (GLOBALSx (cons Gx .. (cons Gy nil) ..)
+     (SEPx (cons (atomic_shift(B := unit) (fun x => S2) (⊤ ∖ E) ∅ (fun x _ => fold_right_sepcon (cons SQx%logic .. (cons SQy%logic nil) ..)) (fun _ => Q)) nil))))))) ..)))
+   (fun (ts: list Type) => rev_curry (tcurry (fun x1 => .. (tcurry (fun xn => tcurry (fun (Q : mpred) (_ : tuple_type tnil) =>
+     PROP () (LOCALx (cons LQx .. (cons LQy nil) ..) (SEPx (Q :: nil)))))) ..)))
+   (@atomic_spec_nonexpansive_pre0 _ W
+      (fun (ts: list Type) => rev_curry (tcurry (fun x1 => .. (tcurry (fun xn (_ : tuple_type tnil) => nil)) ..)))
+      (fun (ts: list Type) => rev_curry (tcurry (fun x1 => .. (tcurry (fun xn (_ : tuple_type tnil) => nil)) ..)))
+      (fun (ts: list Type) => rev_curry (tcurry (fun x1 => .. (tcurry (fun xn (_ : tuple_type tnil) => (cons Gx .. (cons Gy nil) ..))) ..)))
+      (fun (ts: list Type) => rev_curry (tcurry (fun x1 => .. (tcurry (fun xn (_ : tuple_type tnil) => nil)) ..)))
+      (fun (ts: list Type) => rev_curry (tcurry (fun x1 => .. (tcurry (fun xn (_ : tuple_type tnil) x => S2)) ..))) E
+      (fun (ts: list Type) => rev_curry (tcurry (fun x1 => .. (tcurry (fun xn (_ : tuple_type tnil) x _ => fold_right_sepcon (cons SQx%logic .. (cons SQy%logic nil) ..))) ..)))
+     _ _ _ _ _ _)
+  (atomic_spec_nonexpansive_post0 W
+      (fun (ts: list Type) => rev_curry (tcurry (fun x1 => .. (tcurry (fun xn (_ : tuple_type tnil) => (cons LQx%assert3 .. (cons LQy%assert3 nil) ..))) ..)))
+      (fun (ts: list Type) => rev_curry (tcurry (fun x1 => .. (tcurry (fun xn (_ : tuple_type tnil) => nil)) ..))) _ _))
+  (at level 200, x1 closed binder, xn closed binder, x at level 0, E at level 0, S2 at level 0).
+
+Notation "'ATOMIC' 'TYPE' W 'OBJ' x 'INVS' E 'WITH' x1 , .. , xn 'PRE'  [ ] 'PROP' () 'PARAMS' () 'GLOBALS' ( Gx ; .. ; Gy ) 'SEP' () '|' S2 'POST' [ tz ] 'PROP' () 'LOCAL' () 'SEP' () '|' ( SQx ; .. ; SQy )" :=
+  (mk_funspec (pair nil tz) cc_default (atomic_spec_type0 W)
+   (fun (ts: list Type) => rev_curry (tcurry (fun x1 => .. (tcurry (fun xn => tcurry (fun (Q : mpred) (_ : tuple_type tnil) =>
+     PROPx nil
+     (PARAMSx nil (GLOBALSx (cons Gx .. (cons Gy nil) ..)
+     (SEPx (cons (atomic_shift(B := unit) (fun x => S2) (⊤ ∖ E) ∅ (fun x _ => fold_right_sepcon (cons SQx%logic .. (cons SQy%logic nil) ..)) (fun _ => Q)) nil))))))) ..)))
+   (fun (ts: list Type) => rev_curry (tcurry (fun x1 => .. (tcurry (fun xn => tcurry (fun (Q : mpred) (_ : tuple_type tnil) =>
+     PROP () LOCAL () (SEPx (Q :: nil))))) ..)))
+   (@atomic_spec_nonexpansive_pre0 _ W
+      (fun (ts: list Type) => rev_curry (tcurry (fun x1 => .. (tcurry (fun xn (_ : tuple_type tnil) => nil)) ..)))
+      (fun (ts: list Type) => rev_curry (tcurry (fun x1 => .. (tcurry (fun xn (_ : tuple_type tnil) => nil)) ..)))
+      (fun (ts: list Type) => rev_curry (tcurry (fun x1 => .. (tcurry (fun xn (_ : tuple_type tnil) => (cons Gx .. (cons Gy nil) ..))) ..)))
+      (fun (ts: list Type) => rev_curry (tcurry (fun x1 => .. (tcurry (fun xn (_ : tuple_type tnil) => nil)) ..)))
+      (fun (ts: list Type) => rev_curry (tcurry (fun x1 => .. (tcurry (fun xn (_ : tuple_type tnil) x => S2)) ..))) E
+      (fun (ts: list Type) => rev_curry (tcurry (fun x1 => .. (tcurry (fun xn (_ : tuple_type tnil) x _ => fold_right_sepcon (cons SQx%logic .. (cons SQy%logic nil) ..))) ..)))
+     _ _ _ _ _ _)
+  (atomic_spec_nonexpansive_post0 W
+      (fun (ts: list Type) => rev_curry (tcurry (fun x1 => .. (tcurry (fun xn (_ : tuple_type tnil) => nil)) ..)))
+      (fun (ts: list Type) => rev_curry (tcurry (fun x1 => .. (tcurry (fun xn (_ : tuple_type tnil) => nil)) ..))) _ _))
   (at level 200, x1 closed binder, xn closed binder, x at level 0, E at level 0, S2 at level 0).
 
 Notation "'ATOMIC' 'TYPE' W 'INVS' E 'WITH' x1 , .. , xn 'PRE'  [ u , .. , v ] 'PROP' () 'PARAMS' ( Lx ; .. ; Ly ) 'GLOBALS' ( Gx ; .. ; Gy ) 'SEP' ( S1x ; .. ; S1y ) '|' S2 'POST' [ tz ] 'PROP' () 'LOCAL' () 'SEP' ( SPx ; .. ; SPy ) '|' ( SQx ; .. ; SQy )" :=
@@ -961,6 +1003,48 @@ Notation "'ATOMIC' 'TYPE' W 'OBJ' x 'INVS' E 'WITH' x1 , .. , xn 'PRE'  [ u , ..
   (atomic_spec_nonexpansive_post0 W
       (fun (ts: list Type) => rev_curry (tcurry (fun x1 => .. (tcurry (fun xn (_ : tuple_type tnil) => nil)) ..)))
       (fun (ts: list Type) => rev_curry (tcurry (fun x1 => .. (tcurry (fun xn (_ : tuple_type tnil) => (cons SPx%assert5%assert3 .. (cons SPy%assert5%assert3 nil) ..))) ..))) _ _))
+  (at level 200, x1 closed binder, xn closed binder, x at level 0, E at level 0, S2 at level 0).
+
+Notation "'ATOMIC' 'TYPE' W 'INVS' E 'WITH' x1 , .. , xn 'PRE'  [ u , .. , v ] 'PROP' () 'PARAMS' ( Lx ; .. ; Ly ) 'SEP' () '|' S2 'POST' [ tz ] 'PROP' () 'LOCAL' () 'SEP' () '|' ( SQx ; .. ; SQy )" :=
+  (mk_funspec (pair (cons u%type .. (cons v%type nil) ..) tz) cc_default (atomic_spec_type0 W)
+   (fun (ts: list Type) => rev_curry (tcurry (fun x1 => .. (tcurry (fun xn => tcurry (fun (Q : mpred) (_ : tuple_type tnil) =>
+     PROPx nil
+     (PARAMSx (cons Lx%type .. (cons Ly%type nil) ..) (GLOBALSx nil
+     (SEPx (cons (atomic_shift(B := unit) (fun _ : unit => S2) (⊤ ∖ E) ∅ (fun _ _ => fold_right_sepcon (cons SQx%logic .. (cons SQy%logic nil) ..)) (fun _ => Q)) nil))))))) ..)))
+   (fun (ts: list Type) => rev_curry (tcurry (fun x1 => .. (tcurry (fun xn => tcurry (fun (Q : mpred) (_ : tuple_type tnil) =>
+     PROP () LOCAL () (SEPx (Q :: nil))))) ..)))
+   (@atomic_spec_nonexpansive_pre0 _ W
+      (fun (ts: list Type) => rev_curry (tcurry (fun x1 => .. (tcurry (fun xn (_ : tuple_type tnil) => nil)) ..)))
+      (fun (ts: list Type) => rev_curry (tcurry (fun x1 => .. (tcurry (fun xn (_ : tuple_type tnil) => (cons Lx%type .. (cons Ly%type nil) ..))) ..)))
+      (fun (ts: list Type) => rev_curry (tcurry (fun x1 => .. (tcurry (fun xn (_ : tuple_type tnil) => nil)) ..)))
+      (fun (ts: list Type) => rev_curry (tcurry (fun x1 => .. (tcurry (fun xn (_ : tuple_type tnil) => nil)) ..)))
+      (fun (ts: list Type) => rev_curry (tcurry (fun x1 => .. (tcurry (fun xn (_ : tuple_type tnil) (_:unit) => S2)) ..))) E
+      (fun (ts: list Type) => rev_curry (tcurry (fun x1 => .. (tcurry (fun xn (_ : tuple_type tnil) _ _ => fold_right_sepcon (cons SQx%logic .. (cons SQy%logic nil) ..))) ..)))
+     _ _ _ _ _ _)
+  (atomic_spec_nonexpansive_post0 W
+      (fun (ts: list Type) => rev_curry (tcurry (fun x1 => .. (tcurry (fun xn (_ : tuple_type tnil) => nil)) ..)))
+      (fun (ts: list Type) => rev_curry (tcurry (fun x1 => .. (tcurry (fun xn (_ : tuple_type tnil) => nil)) ..))) _ _))
+  (at level 200, x1 closed binder, xn closed binder, E at level 0, S2 at level 0).
+
+Notation "'ATOMIC' 'TYPE' W 'OBJ' x 'INVS' E 'WITH' x1 , .. , xn 'PRE'  [ u , .. , v ] 'PROP' () 'PARAMS' ( Lx ; .. ; Ly ) 'SEP' () '|' S2 'POST' [ tz ] 'PROP' () 'LOCAL' () 'SEP' () '|' ( SQx ; .. ; SQy )" :=
+  (mk_funspec (pair (cons u%type .. (cons v%type nil) ..) tz) cc_default (atomic_spec_type0 W)
+   (fun (ts: list Type) => rev_curry (tcurry (fun x1 => .. (tcurry (fun xn => tcurry (fun (Q : mpred) (_ : tuple_type tnil) =>
+     PROPx nil
+     (PARAMSx (cons Lx%type .. (cons Ly%type nil) ..) (GLOBALSx nil
+     (SEPx (cons (atomic_shift(B := unit) (fun x => S2) (⊤ ∖ E) ∅ (fun x _ => fold_right_sepcon (cons SQx%logic .. (cons SQy%logic nil) ..)) (fun _ => Q)) nil))))))) ..)))
+   (fun (ts: list Type) => rev_curry (tcurry (fun x1 => .. (tcurry (fun xn => tcurry (fun (Q : mpred) (_ : tuple_type tnil) =>
+     PROP () LOCAL () (SEPx (Q :: nil))))) ..)))
+   (@atomic_spec_nonexpansive_pre0 _ W
+      (fun (ts: list Type) => rev_curry (tcurry (fun x1 => .. (tcurry (fun xn (_ : tuple_type tnil) => nil)) ..)))
+      (fun (ts: list Type) => rev_curry (tcurry (fun x1 => .. (tcurry (fun xn (_ : tuple_type tnil) => (cons Lx%type .. (cons Ly%type nil) ..))) ..)))
+      (fun (ts: list Type) => rev_curry (tcurry (fun x1 => .. (tcurry (fun xn (_ : tuple_type tnil) => nil)) ..)))
+      (fun (ts: list Type) => rev_curry (tcurry (fun x1 => .. (tcurry (fun xn (_ : tuple_type tnil) => nil)) ..)))
+      (fun (ts: list Type) => rev_curry (tcurry (fun x1 => .. (tcurry (fun xn (_ : tuple_type tnil) x => S2)) ..))) E
+      (fun (ts: list Type) => rev_curry (tcurry (fun x1 => .. (tcurry (fun xn (_ : tuple_type tnil) x _ => fold_right_sepcon (cons SQx%logic .. (cons SQy%logic nil) ..))) ..)))
+     _ _ _ _ _ _)
+  (atomic_spec_nonexpansive_post0 W
+      (fun (ts: list Type) => rev_curry (tcurry (fun x1 => .. (tcurry (fun xn (_ : tuple_type tnil) => nil)) ..)))
+      (fun (ts: list Type) => rev_curry (tcurry (fun x1 => .. (tcurry (fun xn (_ : tuple_type tnil) => nil)) ..))) _ _))
   (at level 200, x1 closed binder, xn closed binder, x at level 0, E at level 0, S2 at level 0).
 
 Ltac atomic_nonexpansive_tac := try (let x := fresh "x" in intros ?? x;
